rewrite sketch

Logic/Modal/Normal/Completeness.lean
@@ -1,4 +1,3 @@
-import Logic.Propositional.Basic.Completeness
 import Logic.Modal.Normal.Formula
 import Logic.Modal.Normal.HilbertStyle
 import Logic.Modal.Normal.Semantics
@@ -6,68 +5,115 @@ import Logic.Modal.Normal.Soundness
 
 namespace LO.Modal.Normal
 
-open Finset
-open Formula Context Deduction
+open Finset Set
+open Formula Theory
+open Deduction
 
-variable {α β : Type u} [DecidableEq β]
+attribute [simp] Finset.subset_union_right Finset.subset_union_left
+attribute [simp] Set.insert_subset_iff
 
-namespace Formula
+variable {α β : Type u} [Inhabited α] [DecidableEq β]
+
+def Formula.FrameConsequence (F : Frame α) (Γ : Theory β) (p : Formula β) := ∀ V w, (⊧ᴹ[⟨F, V⟩, w] Γ) → (⊧ᴹ[⟨F, V⟩, w] p)
+notation Γ " ⊨ᴹ[" F "] " p => Formula.FrameConsequence F Γ p
+notation Γ " ⊭ᴹ[" F "] " p => ¬(Γ ⊨ᴹ[F] p)
+
+lemma Formula.FrameConsequence.modus_ponens {F : Frame α} {Γ : Theory β} {p : Formula β} : (Γ ⊨ᴹ[F] p ⟶ q) → (Γ ⊨ᴹ[F] p) → (Γ ⊨ᴹ[F] q) := by
+  intro hpq hp V w h;
+  have hpq := by simpa using hpq V w h;
+  have hp := by simpa using hp V w h;
+  exact hpq hp;
+
+def Formula.FrameClassConsequence (𝔽 : FrameClass α) (Γ : Theory β) (p : Formula β) := ∀ F ∈ 𝔽, Γ ⊨ᴹ[F] p
+notation Γ " ⊨ᴹ[" 𝔽 "] " p => Formula.FrameClassConsequence 𝔽 Γ p
+notation Γ " ⊭ᴹ[" 𝔽 "] " p => ¬(Γ ⊨ᴹ[𝔽] p)
+
+namespace Formula.FrameClassConsequence
+
+lemma modus_ponens {𝔽 : FrameClass α} {Γ : Theory β} {p : Formula β} : (Γ ⊨ᴹ[𝔽] p ⟶ q) → (Γ ⊨ᴹ[𝔽] p) → (Γ ⊨ᴹ[𝔽] q) := by
+  simp [Formula.FrameClassConsequence];
+  intro hpq hp F hF;
+  exact (hpq F hF).modus_ponens (hp F hF);
 
 /-
-@[simp] def FrameConsequence (f : Frame α) (Γ : Context β) (p : Formula β) := ∀ V w, (w ⊧ᴹˢ[⟨f, V⟩] Γ) → (w ⊧ᴹˢ[⟨f, V⟩] p)
-
-notation Γ " ⊨ᴹᶠ[" f "] " p => Formula.FrameConsequence f Γ p
-notation Γ " ⊭ᴹᶠ[" f "] " p => ¬(Γ ⊨ᴹᶠ[f] p)
-
-namespace FrameConsequence
-
-variable {f : Frame α} {Γ Γ' : Context β} {p q : Formula β}
-
-@[simp] lemma def_emptyctx : (∅ ⊨ᴹᶠ[f] p) ↔ (⊧ᴹᶠ[f] p) := by aesop;
-@[simp] lemma axiomK : (Γ ⊨ᴹᶠ[f] AxiomK p q) := by aesop;
-@[simp] lemma weakening : (Γ ⊆ Γ') → (Γ ⊨ᴹᶠ[f] p) → (Γ' ⊨ᴹᶠ[f] p) := by aesop;
-@[simp] lemma modus_ponens : (Γ ⊨ᴹᶠ[f] p ⟶ q) → (Γ ⊨ᴹᶠ[f] p) → (Γ ⊨ᴹᶠ[f] q) := by aesop;
-
-end FrameConsequence
+lemma neg {𝔽 : FrameClass α} {Γ : Theory β} {p : Formula β} : (Γ ⊨ᴹ[𝔽] p) ↔ (Γ ⊭ᴹ[𝔽] ~p) := by
+  constructor;
+  . intro h₁;
+    by_contra h₂;
+    have := h₂.modus_ponens h₁;
+    simp [FrameClassConsequence, FrameConsequence, Satisfies] at this;
+  . intro h;
+    simp [Formula.FrameClassConsequence];
+    intro F hF;
 -/
 
-def Consequence (α) (Λ : AxiomSet β) (Γ : Context β) (p : Formula β) := ∀ f ∈ FrameClass α β Λ, ∀ V w, (w ⊧ᴹˢ[⟨f, V⟩] Γ) → (w ⊧ᴹˢ[⟨f, V⟩] p)
+end Formula.FrameClassConsequence
 
-notation Γ " ⊨ᴹ[" Λ "," α "] " p => Consequence α Λ Γ p
-notation Γ " ⊭ᴹ[" Λ "," α "] " p => ¬(Γ ⊨ᴹ[Λ, α] p)
+@[simp]
+def ExtendedDeducible (Λ) (Γ : Theory β) (p) := ∃ (Δ : Finset (Formula β)), (↑Δ ⊆ Γ) ∧ (Δ ⊢ᴹ[Λ]! p)
+notation:40 Γ " ⊢ᴹ[" Λ "]! " p => ExtendedDeducible Λ Γ p
 
-end Formula
+namespace ExtendedDeducible
+
+lemma axm {Λ : AxiomSet β} {Γ : Theory β} {p} : (p ∈ Γ) → (Γ ⊢ᴹ[Λ]! p) := by
+  intro hp;
+  existsi {p}, (by aesop);
+  exact ⟨(Deduction.axm (by simp))⟩;
+
+lemma modus_ponens {Λ : AxiomSet β} {Γ : Theory β} {p q : Formula β} : (Γ ⊢ᴹ[Λ]! (p ⟶ q)) → (Γ ⊢ᴹ[Λ]! p) → (Γ ⊢ᴹ[Λ]! q) := by
+  intro h₁ h₂;
+  simp [ExtendedDeducible] at h₁ h₂;
+  have ⟨Δ₁, ⟨hΔ₁₁, ⟨hΔ₁₂⟩⟩⟩ := h₁;
+  have ⟨Δ₂, ⟨hΔ₂₁, ⟨hΔ₂₂⟩⟩⟩ := h₂;
+
+  have hpq : (Δ₁ ∪ Δ₂) ⊢ᴹ[Λ] (p ⟶ q) := hΔ₁₂.weakening' (by simp);
+  have hp : (Δ₁ ∪ Δ₂) ⊢ᴹ[Λ] p := hΔ₂₂.weakening' (by simp);
+
+  existsi (Δ₁ ∪ Δ₂), (by aesop);
+  exact ⟨(hpq.modus_ponens hp)⟩
+
+end ExtendedDeducible
+
+@[simp]
+abbrev ExtendedUndeducible (Λ) (Γ : Theory β) (p) := ¬(Γ ⊢ᴹ[Λ]! p)
+notation:40 Γ " ⊬ᴹ[" Λ "]! " p => ExtendedUndeducible Λ Γ p
+
+def Theory.FrameSatisfiable (F : Frame α) (Γ : Theory β) := ∃ V w, ⊧ᴹ[⟨F, V⟩, w] Γ
+
+def Theory.FrameClassSatisfiable (𝔽 : FrameClass α) (Γ : Theory β) := ∃ F ∈ 𝔽, Γ.FrameSatisfiable F
 
 section
 
-variable (Λ : AxiomSet β) (Γ : Context β)
+variable (Λ : AxiomSet β) (Γ : Theory β)
 
-def Maximal := ∀ p, p ∈ Γ ∨ ~p ∈ Γ
+def Maximal := ∀ p, (p ∈ Γ) ∨ (~p ∈ Γ)
 
-def Inconsistent (Γ : Set (Formula β)) := ∃ (Δ : Finset (Formula β)), (↑Δ ⊆ Γ) ∧ (Δ ⊢ᴹ[Λ]! ⊥)
+def Theory.Inconsistent (Γ : Theory β) := Γ ⊢ᴹ[Λ]! ⊥
 
-def Consistent (Γ : Set (Formula β)) := ¬(Inconsistent Λ Γ)
+def Theory.Consistent (Γ : Theory β) := ¬(Inconsistent Λ Γ)
 
-def WeakCompleteness := ∀ (f : Frame α) (p : Formula β), (⊧ᴹᶠ[f] p) → (⊢ᴹ[Λ] p)
+def Formula.Inconsistent (p : Formula β) := Theory.Inconsistent {p}
 
-def Completeness (Λ α) := ∀ Γ (p : Formula β), (Γ ⊨ᴹ[Λ, α] p) → (∃ (Δ : Finset (Formula β)), (↑Δ ⊆ Γ) → (Δ ⊢ᴹ[Λ]! p))
+def Formula.Consistent (p : Formula β) := Theory.Consistent {p}
 
-def FrameClassSatisfiable (Λ α) (Γ : Context β) := ∃ f ∈ FrameClass α β Λ, ∃ V w, w ⊧ᴹˢ[⟨f, V⟩] Γ
+def WeakCompleteness := ∀ (p : Formula β), (⊧ᴹ[(𝔽(Λ) : FrameClass α)] p) → (⊢ᴹ[Λ] p)
+
+def Completeness (𝔽 : FrameClass α) := ∀ (Γ : Theory β) (p : Formula β), (Γ ⊨ᴹ[𝔽] p) → (Γ ⊢ᴹ[Λ]! p)
 
 end
 
 variable {Λ : AxiomSet β}
-variable {Γ : Set (Formula β)} (hConsisΓ : Consistent Λ Γ)
+variable {Γ : Set (Formula β)} (hConsisΓ : Theory.Consistent Λ Γ)
 
 @[simp]
-lemma inconsistent_insert_falsum : Inconsistent Λ (insert ⊥ Γ) := by
-  simp [Inconsistent];
+lemma inconsistent_insert_falsum : Theory.Inconsistent Λ (insert ⊥ Γ) := by
+  simp [Theory.Inconsistent];
   existsi {⊥};
   exact ⟨(by simp), ⟨axm (by simp)⟩⟩;
 
 @[simp]
 lemma consistent_isempty_falsum (Δ : Finset (Formula β)) (hΔ : ↑Δ ⊆ Γ) : IsEmpty (Δ ⊢ᴹ[Λ] ⊥) := by
-  simp [Inconsistent, Consistent] at hConsisΓ;
+  simp [Theory.Inconsistent, Theory.Consistent] at hConsisΓ;
   exact hConsisΓ Δ (by assumption);
 
 lemma consistent_no_falsum : ∀ (Δ : Finset (Formula β)), ↑Δ ⊆ Γ → ⊥ ∉ Δ := by
@@ -82,182 +128,273 @@ lemma consistent_no_falsum' : ⊥ ∉ Γ := by
   apply consistent_no_falsum hConsisΓ {⊥} (by aesop);
   simp;
 
-lemma consistent_neither_provable : ∀ (Δ : Finset (Formula β)), ↑Δ ⊆ Γ → ¬((Δ ⊢ᴹ[Λ]! p) ∧ (Δ ⊢ᴹ[Λ]! ~p)) := by
-  intro Δ hΔ;
-  by_contra hC;
-  have := consistent_isempty_falsum hConsisΓ Δ hΔ;
-  exact this.false (modus_ponens hC.2.some hC.1.some);
+lemma consistent_neither_provable (p) : (Γ ⊬ᴹ[Λ]! p) ∨ (Γ ⊬ᴹ[Λ]! ~p) := by
+  by_contra hC; simp only [not_or] at hC;
 
-lemma consistent_neg_undeducible : ∀ (Δ : Finset (Formula β)), ↑Δ ⊆ Γ → (Δ ⊢ᴹ[Λ]! p) → (Δ ⊬ᴹ[Λ]! ~p) := by
-  intro Δ hΔ hp hn;
-  exact consistent_neither_provable hConsisΓ Δ hΔ ⟨hp, hn⟩;
+  have h₁ := hC.1; simp at h₁;
+  have h₂ := hC.2; simp at h₂;
 
-lemma consistent_neither_included : ∀ (Δ : Finset (Formula β)), ↑Δ ⊆ Γ → ∀ p, ¬(p ∈ Δ ∧ ~p ∈ Δ) := by
-  intro Δ hΔ p;
-  by_contra hC;
-  exact consistent_neither_provable hConsisΓ Δ hΔ ⟨⟨axm hC.1⟩, ⟨axm hC.2⟩⟩;
+  have ⟨x, ⟨hx₁, ⟨hx₂⟩⟩⟩ := h₁;
+  have ⟨y, ⟨hy₁, ⟨hy₂⟩⟩⟩ := h₂;
 
-lemma consistent_subset {Γ₁ Γ₂ : Context β} : (Γ₁ ⊆ Γ₂) → (Consistent Λ Γ₂) → (Consistent Λ Γ₁) := by
+  simp [Theory.Inconsistent, Theory.Consistent] at hConsisΓ;
+  exact hConsisΓ (x ∪ y) (by aesop) |>.false
+    $ modus_ponens (hy₂.weakening' (by simp)) (hx₂.weakening' (by simp));
+
+lemma consistent_subset {Γ₁ Γ₂ : Theory β} : (Γ₁ ⊆ Γ₂) → (Consistent Λ Γ₂) → (Consistent Λ Γ₁) := by
   intro hs hConsisΓ₂ hInconsisΓ₁;
-  simp [Consistent, Inconsistent] at hConsisΓ₂ hInconsisΓ₁;
+  simp [Theory.Consistent, Theory.Inconsistent] at hConsisΓ₂ hInconsisΓ₁;
   have ⟨Δ, hΔ₁, hΔ₂⟩ := hInconsisΓ₁;
-  exact (hConsisΓ₂ Δ (Set.Subset.trans hΔ₁ hs)).false hΔ₂.some;
+  exact hConsisΓ₂ Δ (Set.Subset.trans hΔ₁ hs) |>.false hΔ₂.some;
 
-lemma consistent_insert {Γ : Context β} {p : Formula β} : (Consistent Λ (insert p Γ)) → (Consistent Λ Γ) := consistent_subset (by simp)
+lemma consistent_insert {Γ : Theory β} {p : Formula β} : (Consistent Λ (insert p Γ)) → (Consistent Λ Γ) := consistent_subset (by simp)
 
-lemma neg_consistent_intro_undeducible (hConsis : Consistent Λ (insert (~p) Γ)) : ∀ (Δ : Finset (Formula β)), ↑Δ ⊆ Γ → (Δ ⊬ᴹ[Λ]! p) := by
-  simp [Inconsistent, Consistent] at hConsis;
-  intro Δ hΔ;
-  by_contra hC;
-  suffices (insert (~p) Δ ⊢ᴹ[Λ] ⊥) by
-    have : insert (~p) Δ ⊢ᴹ[Λ]! ⊥ := ⟨this⟩;
-    have : insert (~p) Δ ⊬ᴹ[Λ]! ⊥ := by simpa using hConsis (insert (~p) Δ) (by simpa using Set.insert_subset_insert hΔ);
-    aesop;
-  have h₁ : insert (~p) Δ ⊢ᴹ[Λ] p := weakening' (by simp) hC.some;
-  have h₂ : insert (~p) Δ ⊢ᴹ[Λ] p ⟶ ⊥ := by {
-    have : insert (~p) Δ ⊢ᴹ[Λ] ~p := axm (by simp);
-    simpa [Formula.neg_eq] using this;
-  };
-  exact modus_ponens h₂ h₁;
+lemma not_consequence_iff {𝔽 : FrameClass α} {Γ : Theory β} : (Γ ⊨ᴹ[𝔽] p) ↔ (Theory.FrameClassSatisfiable 𝔽 (insert (~p) Γ)) := by
+  constructor;
+  . intro h;
+    sorry;
+  . intro h;
+    sorry;
 
-lemma undeducible_intro_neg_consistent {Γ} (h : Γ ⊬ᴹ[Λ]! p) : (Consistent Λ (insert (~p) Γ)) := by
-  by_contra hC;
+lemma not_deducible_iff {Γ : Theory β} : (Γ ⊬ᴹ[Λ]! p) ↔ (Consistent Λ (insert (~p) Γ)) := by
+  constructor;
+  . intro h;
+    sorry;
+  . intro h;
+    sorry;
 
-  simp [Consistent, Inconsistent] at hC;
-  have ⟨Δ, hΔ₁, hΔ₂⟩ := hC;
-  admit;
+lemma completeness_def {𝔽 : FrameClass α} : (Completeness Λ 𝔽) ↔ (∀ Γ, Consistent Λ Γ → Theory.FrameClassSatisfiable 𝔽 Γ) := by
+  constructor;
+  . contrapose;
+    admit;
+  . contrapose;
+    admit;
 
-  /-
-  by_cases hp : (~p) ∈ Δ;
-  . have hΔ : Δ = insert (~p) (Δ.erase (~p)) := by aesop;
-    rw [hΔ] at hΔ₁ hΔ₂;
-    have : Γ ⊢ᴹ[Λ] p := modus_ponens (dne Γ p) (by
-      rw [neg_eq, neg];
-      have : Γ ⊢ᴹ[Λ] (~p) ⟶ ⊥ := hΔ₂.some.drop.weakening' (by
-        have := Finset.erase_subset_erase (~p) hΔ₁;
-        have := Finset.erase_ssubset_insert Γ (~p);
-      );
+lemma consistent_false (Δ : Finset (Formula β)) (h : ↑Δ ⊆ Γ) : (Undeducible Λ Δ ⊥) := by
+  simp [Theory.Consistent, Theory.Inconsistent] at hConsisΓ;
+  simpa using (hConsisΓ Δ h);
 
-      simpa using hC.some.drop;
-    );
+def MaximalConsistent (Λ) (Γ : Theory β) := Theory.Consistent Λ Γ ∧ Maximal Γ
 
-  have : Γ ⊢ᴹ[Λ] p := modus_ponens (dne Γ p) (by
-    rw [neg_eq, neg];
-    simpa using hC.some.drop;
-  );
-  exact h ⟨this⟩;
-  -/
+section MaximalConsistent
 
-lemma def_not_FrameclassSatisfiable : (Γ ⊭ᴹ[Λ, α] p) ↔ (FrameClassSatisfiable Λ α (insert (~p) Γ)) := by
-  simp only [FrameClassSatisfiable, Consequence];
-  aesop;
+variable (hMCΓ : MaximalConsistent Λ Γ)
 
-lemma intro_Completeness : (∀ (Γ : Context β), Consistent Λ Γ → FrameClassSatisfiable Λ α Γ) → (Completeness Λ α) := by
-  simp [Completeness];
-  intro h₁ Γ p h₂;
-  have := h₁ Γ;
-  sorry;
-
-  /-
-  intro h f hf Γ p hΓp;
-  suffices Γ ⊭ᴹᶠ[f] p by have := this hΓp; contradiction;
-  exact (def_not_FrameclassSatisfiable ht).mpr (h (insert (~p) Γ) (by sorry)) f hf;
-  -/
-
-/-
-lemma maximal_consistent_modus_ponens (hConsisΓ : Consistent Λ Γ) (hMaximalΓ : Maximal Γ) : (p ∈ Γ) → ((p ⟶ q) ∈ Γ) → (q ∈ Γ) := by
-  intro hp hpq; by_contra hnq;
-  apply consistent_neither_provable hConsisΓ;
-  /-
-  exact consistent_neither_provable hConsisΓ ⟨
-    ⟨modus_ponens (axm hpq) (axm hp)⟩,
-    ⟨axm (show ~q ∈ Γ from have := hMaximalΓ q; by simp_all)⟩
-  ⟩;
-  -/
--/
-
-structure MaximalConsistentTheory (Λ : AxiomSet β) where
-  theory : Context β
-  consistent : Consistent Λ theory
-  maximal : ∀ Δ, Consistent Λ Δ → theory ⊆ Δ → Δ = theory
-
-lemma mct_maximality (Ω : MaximalConsistentTheory Λ) : ∀ p, p ∈ Ω.theory ∨ ~p ∈ Ω.theory := by
-  intro p;
-  by_cases hConsis₁ : Consistent Λ (insert p Ω.theory);
-  . have h := Ω.maximal (insert p Ω.theory) hConsis₁ (by simp);
-    rw [←h];
-    simp;
-  . have h := Ω.maximal (insert (~p) Ω.theory) (by
-      by_contra hConsis₂;
-      simp [Consistent, Inconsistent] at hConsis₁ hConsis₂;
-      have ⟨Δ₁, h₁₁, h₁₂⟩ := hConsis₁;
-      have ⟨Δ₂, h₂₁, h₂₂⟩ := hConsis₂;
-      have : Inconsistent Λ Ω.theory := by sorry;
-      apply Ω.consistent this;
-    ) (by simp);
-    rw [←h];
-    simp;
-  -- have := Ω.maximal (insert p Ω.theory);
-
-lemma axiomset_include (Ω : MaximalConsistentTheory Λ) : Λ ⊆ Ω.theory := by
+lemma axiomset_include : Λ ⊆ Γ := by
   intro p hp;
   by_contra hC;
-  have hConsis := by simpa [Consistent, Inconsistent] using Ω.consistent;
-  have : ~p ∈ Ω.theory := by simpa [hC] using mct_maximality Ω p;
-  have h₂ : {~p} ⊬ᴹ[Λ]! ⊥ := by simpa using hConsis {~p} (by aesop);
-  have h₃ : ⊢ᴹ[Λ] ~~p := by {
-    have : ⊢ᴹ[Λ] p := maxm hp;
-    admit
-  }
-  have : {~p} ⊢ᴹ[Λ] ⊥ := by sorry;
-  exact h₂ ⟨this⟩;
+  apply consistent_false hMCΓ.1 {~p} (by have := hMCΓ.2 p; aesop) ⟨(axm (by simp)).modus_ponens (maxm hp)⟩;
 
-lemma exists_maximal_consistent_theory (hConsisΓ : Consistent Λ Γ) :
-  ∃ Γ', Consistent Λ Γ' ∧ Γ ⊆ Γ' ∧ ∀ Δ, Consistent Λ Δ → Γ' ⊆ Δ → Δ = Γ' :=
-  zorn_subset_nonempty { Γ' | Consistent Λ Γ' } (by
-    intro c hc chain hnc;
-    existsi ⋃₀ c;
-    constructor;
-    . simp;
-      by_contra hC;
-      suffices Consistent Λ (⋃₀ c) by aesop;
-      admit;
-    . apply Set.subset_sUnion_of_mem
-  ) Γ hConsisΓ
+lemma member_of_maximal_consistent : (p ∈ Γ) ↔ (Γ ⊢ᴹ[Λ]! p) := by
+  constructor;
+  . intros; existsi {p}; aesop;
+  . intro h;
+    suffices ~p ∉ Γ by have := hMCΓ.2 p; aesop;
+    by_contra hC;
+    have ⟨Δ, ⟨hΔ₁, ⟨hΔ₂⟩⟩⟩ := h;
+    have : (insert (~p) Δ) ⊢ᴹ[Λ] ⊥ := (axm (by simp)).modus_ponens (hΔ₂.weakening' (by simp));
+    have : ↑(insert (~p) Δ) ⊆ Γ := by simp_all [coe_insert, Set.insert_subset_iff];
+    apply consistent_false hMCΓ.1 _ (by assumption) ⟨(by assumption)⟩;
 
-lemma lindenbaum (hConsisΓ : Consistent Λ Γ) : ∃ (Ω : MaximalConsistentTheory Λ), (Γ ⊆ Ω.theory) := by
-  have ⟨Γ', ⟨hConsisΓ', hΓΓ', hMaximalΓ'⟩⟩ := exists_maximal_consistent_theory hConsisΓ;
-  existsi ⟨Γ', (by assumption), (by assumption)⟩;
-  assumption;
+lemma maximal_consistent_modus_ponens {p q : Formula β} : (p ∈ Γ) → ((p ⟶ q) ∈ Γ) → (q ∈ Γ) := by
+  intro hp hpq;
+  have dp  := (member_of_maximal_consistent hMCΓ).mp hp;
+  have dpq := (member_of_maximal_consistent hMCΓ).mp hpq;
+  exact (member_of_maximal_consistent hMCΓ).mpr $ dpq.modus_ponens dp;
 
-def CanonicalModel (Λ : AxiomSet β) : Model (MaximalConsistentTheory Λ) β where
-  frame (Γ Δ) := ∀ (p : Formula β), (□p ∈ Γ.theory) → (p ∈ Δ.theory)
-  val (Γ a) := (atom a) ∈ Γ.theory
+lemma maximal_neg_include : (~p ∈ Γ) ↔ (p ∉ Γ) := by
+  constructor;
+  . intros;
+    by_contra hC;
+    have hp : ({p, ~p}) ⊢ᴹ[Λ] p := axm (by simp);
+    have hnp : ({p, ~p}) ⊢ᴹ[Λ] ~p := axm (by simp);
+    apply consistent_false hMCΓ.1 {p, ~p} (by aesop;) ⟨hnp.modus_ponens hp⟩;
+  . have := hMCΓ.2 p; aesop;
+
+lemma maximal_imp_include : (p ⟶ q ∈ Γ) ↔ (p ∉ Γ) ∨ (q ∈ Γ) := by
+  constructor;
+  . simp [or_iff_not_imp_left];
+    intros;
+    apply (member_of_maximal_consistent hMCΓ).mpr;
+    have hp : ({p, p ⟶ q}) ⊢ᴹ[Λ] p := axm (by simp);
+    have hpq : ({p, p ⟶ q}) ⊢ᴹ[Λ] p ⟶ q := axm (by simp);
+    have := hpq.modus_ponens hp;
+    existsi {p, p ⟶ q}, (by aesop)
+    exact ⟨hpq.modus_ponens hp⟩;
+  . intros h;
+    cases h;
+    case inl h =>
+      have := (maximal_neg_include hMCΓ).mpr h;
+      have d₁ : Γ ⊢ᴹ[Λ]! (~p ⟶ (p ⟶ q)) := by admit;
+      have d₂ : Γ ⊢ᴹ[Λ]! ~p := by existsi {~p}; aesop;
+      apply (member_of_maximal_consistent hMCΓ).mpr;
+      exact d₁.modus_ponens d₂;
+    case inr h =>
+      have d₁ : Γ ⊢ᴹ[Λ]! (q ⟶ (p ⟶ q)) := by
+        existsi ∅, by simp;
+        exact ⟨imply₁ _ _ _⟩;
+      have d₂ : Γ ⊢ᴹ[Λ]! q := by existsi {q}; aesop;
+      apply (member_of_maximal_consistent hMCΓ).mpr;
+      exact d₁.modus_ponens d₂;
+
+lemma maximal_imp_include' : (p ⟶ q ∈ Γ) ↔ ((p ∈ Γ) → (q ∈ Γ)) := by
+  constructor;
+  . intro hpq hp;
+    have := (maximal_imp_include hMCΓ).mp hpq;
+    aesop;
+  . intro hp;
+    apply (maximal_imp_include hMCΓ).mpr;
+    simp [or_iff_not_imp_left];
+    aesop;
+
+end MaximalConsistent
+
+structure MaximalConsistentTheory (Λ : AxiomSet β) where
+  theory : Theory β
+  consistent : Consistent Λ theory
+  maximal : Maximal theory
+
+namespace MaximalConsistentTheory
 
 @[simp]
-lemma CanonicalModel_frame {Λ : AxiomSet β} {Ω MΔ : MaximalConsistentTheory Λ} :
-  (CanonicalModel Λ).frame Ω MΔ ↔ (∀ (p : Formula β), (□p ∈ Ω.theory) → (p ∈ MΔ.theory))
+def membership (p : Formula β) (Ω : MaximalConsistentTheory Λ) := p ∈ Ω.theory
+instance : Membership (Formula β) (MaximalConsistentTheory Λ) := ⟨membership⟩
+
+@[simp]
+def subset (Ω₁ Ω₂ : MaximalConsistentTheory Λ) := Ω₁.theory ⊆ Ω₂.theory
+instance : HasSubset (MaximalConsistentTheory Λ) := ⟨subset⟩
+
+@[simp]
+def subset' (Γ : Theory β) (Ω : MaximalConsistentTheory Λ) := Γ ⊆ Ω.theory
+infix:50 "⊆" => subset'
+
+@[simp]
+lemma mc (Ω : MaximalConsistentTheory Λ) : MaximalConsistent Λ Ω.theory := by
+  constructor;
+  . exact Ω.consistent;
+  . exact Ω.maximal;
+
+end MaximalConsistentTheory
+
+section Lindenbaum
+
+variable (Λ : AxiomSet β)
+variable [∀ Γ p, Decidable (Consistent Λ (insert p Γ))]
+variable [Denumerable (Formula β)]
+
+open Encodable Denumerable
+
+def lindenbaum_step (Γ : Theory β) (p : Formula β) : Theory β :=
+  if Consistent Λ (insert p Γ) then (insert p Γ) else insert (~p) Γ
+
+lemma lindenbaum_step_include (Γ : Theory β) : ∀ p, (p ∈ lindenbaum_step Λ Γ p) ∨ (~p ∈ lindenbaum_step Λ Γ p) := by
+  intro p;
+  simp [lindenbaum_step];
+  by_cases hConsis : Consistent Λ (insert p Γ) <;> aesop;
+
+@[simp]
+lemma lindenbaum_step_subset (Γ : Theory β) (p : Formula β) : Γ ⊆ lindenbaum_step Λ Γ p := by
+  simp only [lindenbaum_step];
+  by_cases hConsis : Consistent Λ (insert p Γ) <;> aesop;
+
+def lindenbaum_set (Γ : Theory β) : ℕ → (Theory β)
+  | .zero => Γ
+  | .succ n => lindenbaum_step Λ (lindenbaum_set Γ n) (ofNat _ n)
+
+notation Γ "[" Λ ", " i "]" => lindenbaum_set Λ Γ i
+
+@[simp]
+lemma lindenbaum_set_zero (Γ : Theory β) : Γ[Λ, 0] = Γ := rfl
+
+@[simp]
+lemma lindenbaum_set_succ (Γ : Theory β) (n : ℕ) : Γ[Λ, n + 1] = lindenbaum_step Λ (Γ[Λ, n]) (ofNat _ n) := rfl
+
+lemma lindenbaum_set_subset_next (Γ : Theory β) : ∀ n, Γ[Λ, n] ⊆ Γ[Λ, n + 1] := by aesop;
+
+lemma lindenbaum_set_consistent (Γ : Theory β) (hConsisΓ : Consistent Λ Γ) : ∀ n, Consistent Λ (Γ[Λ, n]) := by
+  intro n;
+  induction n with
+  | zero => simpa;
+  | succ n ih =>
+    simp only [lindenbaum_set, lindenbaum_step];
+    split;
+    case inl => assumption;
+    case inr hInconsis₁ => sorry
+      /-
+      by_contra hInconsis₂;
+      simp [Consistent, Inconsistent, -NegDefinition.neg] at hInconsis₁ hInconsis₂;
+      have ⟨Δ₁, ⟨hΔ₁₁, ⟨hΔ₁₂⟩⟩⟩ := hInconsis₁;
+      have ⟨Δ₂, ⟨hΔ₂₁, ⟨hΔ₂₂⟩⟩⟩ := hInconsis₂;
+      -/
+
+lemma lindenbaum_set_maximal (Γ : Theory β) : ∀ (p : Formula β), p ∈ Γ[Λ, (encode p)] ∨ (~p ∈ Γ[Λ, (encode p)]) := by
+  intro p;
+  sorry;
+
+def lindenbaum_set_iUnion (Γ : Theory β) := iUnion (lindenbaum_set Λ Γ)
+notation Γ "[" Λ "]⁺" => lindenbaum_set_iUnion Λ Γ
+
+lemma lindenbaum_set_iUnion_maximal (Γ : Theory β) : ∀ (p : Formula β), p ∈ Γ[Λ]⁺ ∨ ~p ∈ Γ[Λ]⁺ := by
+  intro p;
+  simp [lindenbaum_set_iUnion, -NegDefinition.neg];
+  cases lindenbaum_set_maximal Λ Γ p;
+  case inl h => left; existsi (encode p); assumption;
+  case inr h => right; existsi (encode p); assumption;
+
+lemma lindenbaum_set_iUnion_subset_original (Γ : Theory β) : Γ ⊆ Γ[Λ]⁺ := by
+  intro p hp;
+  simp [lindenbaum_set_iUnion];
+  existsi 0;
+  simpa;
+
+lemma lindenbaum (hConsisΓ : Consistent Λ Γ) : ∃ (Ω : Theory β), (Γ ⊆ Ω) ∧ (MaximalConsistent Λ Ω) := by
+  existsi Γ[Λ]⁺;
+  constructor;
+  . apply lindenbaum_set_iUnion_subset_original;
+  . constructor;
+    . admit;
+    . apply lindenbaum_set_iUnion_maximal;
+
+lemma lindenbaum' (hConsisΓ : Consistent Λ Γ) : ∃ (Ω : MaximalConsistentTheory Λ), (Γ ⊆ Ω) := by
+  have ⟨Ω, hΩ⟩ := lindenbaum Λ hConsisΓ;
+  existsi ⟨Ω, hΩ.2.1, hΩ.2.2⟩;
+  exact hΩ.1;
+
+end Lindenbaum
+
+def CanonicalModel (Λ : AxiomSet β) : Model (MaximalConsistentTheory Λ) β where
+  frame (Ω₁ Ω₂) := ∀ (p : Formula β), (□p ∈ Ω₁) → (p ∈ Ω₂)
+  val (Ω a) := (atom a) ∈ Ω
+
+@[simp]
+lemma CanonicalModel_frame {Λ : AxiomSet β} {Ω₁ Ω₂ : MaximalConsistentTheory Λ} :
+  (CanonicalModel Λ).frame Ω₁ Ω₂ ↔ (∀ (p : Formula β), (□p ∈ Ω₁) → (p ∈ Ω₂))
   := by rfl
 
 @[simp]
 lemma CanonicalModel_val {Λ : AxiomSet β} {Ω : MaximalConsistentTheory Λ} {a : β} :
-  a ∈ (CanonicalModel Λ).val Ω ↔ (atom a) ∈ Ω.theory
+  a ∈ (CanonicalModel Λ).val Ω ↔ (atom a) ∈ Ω
   := by rfl
 
-lemma mem_maximalConsistentTheory_iff
-  {Ω : MaximalConsistentTheory Λ} {p : Formula β} : (Ω ⊧ᴹˢ[CanonicalModel Λ] p) ↔ (p ∈ Ω.theory) := by
+lemma truthlemma {Ω : MaximalConsistentTheory Λ} {p : Formula β} : (⊧ᴹ[CanonicalModel Λ, Ω] p) ↔ (p ∈ Ω) := by
   induction p using rec' with
-  | hatom a => simp;
+  | hatom a => aesop;
   | hfalsum => simpa [Satisfies.bot_def] using consistent_no_falsum' Ω.consistent;
   | himp p q ihp ihq =>
-    simp [ihp, ihq];
+    -- simp [ihp, ihq];
     constructor;
     . intro h;
+      admit
+    . intros;
       sorry;
-    . intro hpq hp;
-      sorry;
-  | hor p q ih => sorry;
-  | hand p q ihp ihq => sorry;
+  | hor p q ih =>
+    constructor;
+    . intro h; sorry;
+    . intro h; sorry;
+  | hand p q ihp ihq =>
+    constructor;
+    . intro h; sorry;
+    . intro h; sorry;
   | hbox p ih =>
     constructor;
     . contrapose;
@@ -267,24 +404,26 @@ lemma mem_maximalConsistentTheory_iff
       have b := h₂ _ h;
       sorry;
 
-
-lemma mem_maximalConsistentTheory_iff'
-  {Ω : MaximalConsistentTheory Λ} {Γ : Context β} : (Ω ⊧ᴹˢ[CanonicalModel Λ] Γ) ↔ (Γ ⊆ Ω.theory) := by
-  simp [Set.subset_def];
+lemma truthlemma' {Ω : MaximalConsistentTheory Λ} {Γ : Theory β} : (⊧ᴹ[CanonicalModel Λ, Ω] Γ) ↔ (Γ ⊆ Ω) := by
   constructor;
-  . intro h p hp; exact (mem_maximalConsistentTheory_iff).mp (h p hp);
-  . intro h p hp; exact (mem_maximalConsistentTheory_iff).mpr (h p hp);
+  . simp [Set.subset_def];
+    intro h p hp;
+    exact truthlemma.mp $ h p hp;
+  . intro h p hp;
+    apply truthlemma.mpr;
+    aesop;
 
-theorem LogicK.Hilbert.completes : Completeness (𝐊 : AxiomSet β) (MaximalConsistentTheory (𝐊 : AxiomSet β)) := by
-  apply intro_Completeness;
+variable [∀ Λ Γ p, Decidable (Consistent (Λ : AxiomSet β) (insert p Γ))] [Denumerable (Formula β)]
 
+theorem LogicK.Hilbert.completes : Completeness (𝐊 : AxiomSet β) (𝔽((𝐊 : AxiomSet β)) : FrameClass (MaximalConsistentTheory (𝐊 : AxiomSet β)) ) := by
+  apply completeness_def.mpr;
   intro Γ hConsisΓ;
-  let ⟨Ω, hΩ⟩ := lindenbaum hConsisΓ;
-
+  let ⟨Ω, hΩ⟩ := lindenbaum' (𝐊 : AxiomSet β) hConsisΓ;
   existsi (CanonicalModel 𝐊).frame;
   constructor;
   . apply LogicK.def_FrameClass;
   . existsi (CanonicalModel 𝐊).val, Ω;
-    apply mem_maximalConsistentTheory_iff'.mpr hΩ;
+    apply truthlemma'.mpr;
+    assumption;
 
 end LO.Modal.Normal
